tools/auto/experiments/test3.lean
@@ -5,46 +5,46 @@ Authors: Jeremy Avigad
 
 Examples from the tutorial.
 -/
-import .auto
-open tactic
+import ..finish
+open auto
 
 section
 variables p q r s : Prop
 
 -- commutativity of ∧ and ∨
-example : p ∧ q ↔ q ∧ p := by safe'
-example : p ∨ q ↔ q ∨ p := by safe'
+example : p ∧ q ↔ q ∧ p := by finish
+example : p ∨ q ↔ q ∨ p := by finish
 
 -- associativity of ∧ and ∨
-example : (p ∧ q) ∧ r ↔ p ∧ (q ∧ r) := by safe'
-example : (p ∨ q) ∨ r ↔ p ∨ (q ∨ r) := by safe'
+example : (p ∧ q) ∧ r ↔ p ∧ (q ∧ r) := by finish
+example : (p ∨ q) ∨ r ↔ p ∨ (q ∨ r) := by finish
 
 -- distributivity
-example : p ∧ (q ∨ r) ↔ (p ∧ q) ∨ (p ∧ r) := by safe'
-example : p ∨ (q ∧ r) ↔ (p ∨ q) ∧ (p ∨ r) := by safe'
+example : p ∧ (q ∨ r) ↔ (p ∧ q) ∨ (p ∧ r) := by finish [iff_def]
+example : p ∨ (q ∧ r) ↔ (p ∨ q) ∧ (p ∨ r) := by finish
 
 -- other properties
-example : (p → (q → r)) ↔ (p ∧ q → r) := by safe'
-example : ((p ∨ q) → r) ↔ (p → r) ∧ (q → r) := by safe'
-example : ¬(p ∨ q) ↔ ¬p ∧ ¬q := by safe'
-example : ¬p ∨ ¬q → ¬(p ∧ q) := by safe'
-example : ¬(p ∧ ¬ p) := by safe'
-example : p ∧ ¬q → ¬(p → q) := by safe'
-example : ¬p → (p → q) := by safe'
-example : (¬p ∨ q) → (p → q) := by safe'
-example : p ∨ false ↔ p := by safe'
-example : p ∧ false ↔ false := by safe'
-example : ¬(p ↔ ¬p) := by safe'
-example : (p → q) → (¬q → ¬p) := by safe'
+example : (p → (q → r)) ↔ (p ∧ q → r) := by finish
+example : ((p ∨ q) → r) ↔ (p → r) ∧ (q → r) := by finish
+example : ¬(p ∨ q) ↔ ¬p ∧ ¬q := by finish
+example : ¬p ∨ ¬q → ¬(p ∧ q) := by finish
+example : ¬(p ∧ ¬ p) := by finish
+example : p ∧ ¬q → ¬(p → q) := by finish
+example : ¬p → (p → q) := by finish
+example : (¬p ∨ q) → (p → q) := by finish
+example : p ∨ false ↔ p := by finish
+example : p ∧ false ↔ false := by finish
+example : ¬(p ↔ ¬p) := by finish
+example : (p → q) → (¬q → ¬p) := by finish
 
 -- these require classical reasoning
-example : (p → r ∨ s) → ((p → r) ∨ (p → s)) := by safe'
-example : ¬(p ∧ q) → ¬p ∨ ¬q := by safe'
-example : ¬(p → q) → p ∧ ¬q := by safe'
-example : (p → q) → (¬p ∨ q) := by safe'
-example : (¬q → ¬p) → (p → q) := by safe'
-example : p ∨ ¬p := by safe'
-example : (((p → q) → p) → p) := by safe'
+example : (p → r ∨ s) → ((p → r) ∨ (p → s)) := by finish
+example : ¬(p ∧ q) → ¬p ∨ ¬q := by finish
+example : ¬(p → q) → p ∧ ¬q := by finish
+example : (p → q) → (¬p ∨ q) := by finish
+example : (¬q → ¬p) → (p → q) := by finish
+example : p ∨ ¬p := by finish
+example : (((p → q) → p) → p) := by finish
 end
 
 /- to get the ones that are sorried, we need to find an element in the environment
@@ -56,27 +56,36 @@ variables (A : Type) (p q : A → Prop)
 variable a : A
 variable r : Prop
 
-example : (∃ x : A, r) → r := by auto'
---example : r → (∃ x : A, r) := by auto'
-example : (∃ x, p x ∧ r) ↔ (∃ x, p x) ∧ r := by auto'
+example : (∃ x : A, r) → r := by finish
+--example : r → (∃ x : A, r) := by finish
+example : (∃ x, p x ∧ r) ↔ (∃ x, p x) ∧ r := by finish
 
-example : (∃ x, p x ∨ q x) ↔ (∃ x, p x) ∨ (∃ x, q x) := by auto'
+theorem foo: (∃ x, p x ∨ q x) ↔ (∃ x, p x) ∨ (∃ x, q x) := 
+begin 
+  simp [iff_def], 
+  trace "hello",
+  auto.preprocess_goal {},
+  auto.preprocess_hyps {},
+  trace "goodbye"
+end
 
-example (h : ∀ x, ¬ ¬ p x) : p a := by force'
-example (h : ∀ x, ¬ ¬ p x) : ∀ x, p x := by auto'
+#exit
 
-example : (∀ x, p x) ↔ ¬ (∃ x, ¬ p x) := by auto'
+example (h : ∀ x, ¬ ¬ p x) : p a := by finish
+example (h : ∀ x, ¬ ¬ p x) : ∀ x, p x := by finish
 
-example : (∃ x, p x) ↔ ¬ (∀ x, ¬ p x) := sorry
-example : (¬ ∃ x, p x) ↔ (∀ x, ¬ p x) := by auto'
-example : (¬ ∀ x, p x) ↔ (∃ x, ¬ p x) := sorry
-example : (∃ x, ¬ p x) → (¬ ∀ x, p x) := by auto'
+example : (∀ x, p x) ↔ ¬ (∃ x, ¬ p x) := by finish
 
-example : (∀ x, p x → r) ↔ (∃ x, p x) → r := by auto'
-example : (∃ x, p x → r) ↔ (∀ x, p x) → r := sorry
-example : (∃ x, r → p x) ↔ (r → ∃ x, p x) := sorry
+example : (∃ x, p x) ↔ ¬ (∀ x, ¬ p x) := by finish
+example : (¬ ∃ x, p x) ↔ (∀ x, ¬ p x) := by finish
+example : (¬ ∀ x, p x) ↔ (∃ x, ¬ p x) := by finish
+example : (∃ x, ¬ p x) → (¬ ∀ x, p x) := by finish
+/-
+example : (∀ x, p x → r) ↔ (∃ x, p x) → r := by finish [iff_def]
+example : (∃ x, p x → r) ↔ (∀ x, p x) → r := begin safe [iff_def] end -- by finish [iff_def]
+example : (∃ x, r → p x) ↔ (r → ∃ x, p x) := by finish [iff_def]
 
-example : (∃ x, p x → r) → (∀ x, p x) → r := by auto'
-example : (∃ x, r → p x) → (r → ∃ x, p x) := by auto'
-
+example : (∃ x, p x → r) → (∀ x, p x) → r := by finish
+example : (∃ x, r → p x) → (r → ∃ x, p x) := by finish
+-/
 end
